theories/Reflection2/OrderedType.v
@@ -19,21 +19,21 @@ type inference work properly... *)
 
 Class OType (A:Type) : Type :=
   {
-    ot_R : relation A;
-    ot_PreOrder :> PreOrder ot_R
+    oleq : relation A;
+    oPreOrder :> PreOrder oleq
   }.
 
-Instance OType_Reflexive A `{OType A} : Reflexive ot_R.
+Instance OType_Reflexive A `{OType A} : Reflexive oleq.
 Proof. typeclasses eauto. Qed.
 
-Instance OType_Transitive A `{OType A} : Transitive ot_R.
+Instance OType_Transitive A `{OType A} : Transitive oleq.
 Proof. typeclasses eauto. Qed.
 
 (* The equivalence relation for an OrderedType *)
-Definition ot_equiv {A} `{OType A} : relation A :=
-  fun x y => ot_R x y /\ ot_R y x.
+Definition oeq {A} `{OType A} : relation A :=
+  fun x y => oleq x y /\ oleq y x.
 
-Instance ot_equiv_Equivalence A `{OType A} : Equivalence ot_equiv.
+Instance oeq_Equivalence A `{OType A} : Equivalence oeq.
 Proof.
   constructor; intro; intros.
   { split; reflexivity. }
@@ -42,42 +42,42 @@ Proof.
 Qed.
 
 Notation "x <o= y" :=
-  (ot_R x y) (no associativity, at level 70).
+  (oleq x y) (no associativity, at level 70).
 Notation "x =o= y" :=
-  (ot_equiv x y) (no associativity, at level 70).
+  (oeq x y) (no associativity, at level 70).
 
-(* FIXME: replace "ot_R" below with "<o=" notation *)
+(* FIXME: replace "oleq" below with "<o=" notation *)
 
 (* FIXME: figure out what versions of this we need for rewriting! *)
-Instance Proper_ot_R_ot_R A `{OType A}
-  : Proper (ot_R --> ot_R ==> Basics.impl) (@ot_R A _).
+Instance Proper_oleq_oleq A `{OType A}
+  : Proper (oleq --> oleq ==> Basics.impl) (@oleq A _).
 Proof.
   intros a1 a2 Ra b1 b2 Rb Rab.
   transitivity a1; [ assumption | ]. transitivity b1; assumption.
 Qed.
 
-Instance Subrelation_ot_equiv_ot_R A `{OType A} :
-  subrelation (@ot_equiv A _) ot_R.
+Instance Subrelation_oeq_oleq A `{OType A} :
+  subrelation (@oeq A _) oleq.
 Proof.
   intros a1 a2 Ra; destruct Ra; assumption.
 Qed.
 
-Instance Proper_ot_equiv_ot_R A `{OType A} :
-  Proper (ot_equiv ==> ot_equiv ==> iff) (@ot_R A _).
+Instance Proper_oeq_oleq A `{OType A} :
+  Proper (oeq ==> oeq ==> iff) (@oleq A _).
 Proof.
   intros x1 x2 Rx y1 y2 Ry; destruct Rx; destruct Ry; split; intro Rxy.
   transitivity x1; [ assumption | ]; transitivity y1; assumption.
   transitivity x2; [ assumption | ]; transitivity y2; assumption.
 Qed.
 
-Instance Proper_ot_equiv A `{OType A} :
-  Proper (ot_equiv ==> ot_equiv ==> iff) (@ot_equiv A _).
+Instance Proper_oeq A `{OType A} :
+  Proper (oeq ==> oeq ==> iff) (@oeq A _).
 Proof.
   intros x1 x2 Rx y1 y2 Ry. rewrite Rx. rewrite Ry. reflexivity.
 Qed.
 
-Instance Proper_ot_equiv_partial A `{OType A} a :
-  Proper (ot_equiv ==> Basics.flip Basics.impl) (@ot_equiv A _ a).
+Instance Proper_oeq_partial A `{OType A} a :
+  Proper (oeq ==> Basics.flip Basics.impl) (@oeq A _ a).
 Proof.
   intros x1 x2 Rx. rewrite Rx. reflexivity.
 Qed.
@@ -89,12 +89,12 @@ Qed.
 
 (* The ordered type of propositions *)
 Instance OTProp : OType Prop :=
-  {| ot_R := Basics.impl |}.     
+  {| oleq := Basics.impl |}.     
 Proof. repeat constructor; typeclasses eauto. Defined.
 
 (* Proofs are always related (i.e., this is the proof irrelevance type) *)
 Instance OTproof (P:Prop) : OType P :=
-  {| ot_R := fun _ _ => True |}.
+  {| oleq := fun _ _ => True |}.
 Proof.
   repeat constructor.
 Defined.
@@ -102,7 +102,7 @@ Defined.
 (* The discrete ordered type, where things are only related to themselves; we
 make this a definition, not an instance, so that it can be instantiated for
 particular types. *)
-Definition OTdiscrete A : OType A := {| ot_R := eq |}.
+Definition OTdiscrete A : OType A := {| oleq := eq |}.
 
 (* The only ordered type over unit is the discrete one *)
 Instance OTunit : OType unit := OTdiscrete unit.
@@ -115,7 +115,7 @@ Arguments flip {A} a.
 Definition unflip {A} (f:Flip A) : A := let (x) := f in x.
 
 Instance OTFlip A (R:OType A) : OType (Flip A) :=
-  {| ot_R := fun x y => unflip y <o= unflip x |}.
+  {| oleq := fun x y => unflip y <o= unflip x |}.
 Proof.
   repeat constructor; intro; intros.
   - destruct x; compute; reflexivity.
@@ -127,7 +127,7 @@ Instance OTbool : OType bool := OTdiscrete bool.
 
 (* The pointwise relation on pairs *)
 Instance OTpair A B `(OType A) `(OType B) : OType (A*B) :=
-  {| ot_R := fun p1 p2 => ot_R (fst p1) (fst p2) /\ ot_R (snd p1) (snd p2) |}.
+  {| oleq := fun p1 p2 => oleq (fst p1) (fst p2) /\ oleq (snd p1) (snd p2) |}.
 Proof.
   repeat constructor.
   - destruct x. reflexivity.
@@ -141,11 +141,11 @@ Defined.
 
 (* The sort-of pointwise relation on sum types *)
 Inductive sumR {A B} (RA:OType A) (RB:OType B) : A+B -> A+B -> Prop :=
-| sumR_inl a1 a2 : ot_R a1 a2 -> sumR RA RB (inl a1) (inl a2)
-| sumR_inr b1 b2 : ot_R b1 b2 -> sumR RA RB (inr b1) (inr b2).
+| sumR_inl a1 a2 : oleq a1 a2 -> sumR RA RB (inl a1) (inl a2)
+| sumR_inr b1 b2 : oleq b1 b2 -> sumR RA RB (inr b1) (inr b2).
 
 Instance OTsum A B (RA:OType A) (RB:OType B) : OType (A+B) :=
-  {| ot_R := sumR RA RB |}.
+  {| oleq := sumR RA RB |}.
 Proof.
   repeat constructor; intro; intros.
   { destruct x; constructor; reflexivity. }
@@ -165,11 +165,11 @@ UIP to hold if we want to use the definition given here... *)
 Program Definition OTType : OType :=
   {|
     ot_Type := OType;
-    ot_R := (fun A B =>
+    oleq := (fun A B =>
                exists (e:ot_Type A = ot_Type B),
                  forall (x y:A),
-                   ot_R A x y ->
-                   ot_R B (rew [fun A => A] e in x)
+                   oleq A x y ->
+                   oleq B (rew [fun A => A] e in x)
                         (rew [fun A => A] e in y));
   |}.
 *)
@@ -180,38 +180,38 @@ Program Definition OTType : OType :=
  ***)
 
 Instance Proper_pair A B `{OType A} `{OType B} :
-  Proper (ot_R ==> ot_R ==> ot_R) (pair : A -> B -> A*B).
+  Proper (oleq ==> oleq ==> oleq) (pair : A -> B -> A*B).
 Proof.
   repeat intro; split; assumption.
 Qed.
 
 Instance Proper_pair_equiv A B `{OType A} `{OType B} :
-  Proper (ot_equiv ==> ot_equiv ==> ot_equiv) (pair : A -> B -> A*B).
+  Proper (oeq ==> oeq ==> oeq) (pair : A -> B -> A*B).
 Proof.
   intros a1 a2 Ra b1 b2 Rb; destruct Ra; destruct Rb; split; split; assumption.
 Qed.
 
 Instance Proper_fst A B `{OType A} `{OType B} :
-  Proper (ot_R ==> ot_R) (fst : A*B -> A).
+  Proper (oleq ==> oleq) (fst : A*B -> A).
 Proof.
   intros p1 p2 Rp; destruct Rp; assumption.
 Qed.
 
 Instance Proper_fst_equiv A B `{OType A} `{OType B} :
-  Proper (ot_equiv ==> ot_equiv) (fst : A*B -> A).
+  Proper (oeq ==> oeq) (fst : A*B -> A).
 Proof.
   intros p1 p2 Rp. destruct Rp.
   split; eapply Proper_fst; assumption.
 Qed.
 
 Instance Proper_snd A B `{OType A} `{OType B} :
-  Proper (ot_R ==> ot_R) (snd : A*B -> B).
+  Proper (oleq ==> oleq) (snd : A*B -> B).
 Proof.
   intros p1 p2 Rp; destruct Rp; assumption.
 Qed.
 
 Instance Proper_snd_equiv A B `{OType A} `{OType B} :
-  Proper (ot_equiv ==> ot_equiv) (snd : A*B -> B).
+  Proper (oeq ==> oeq) (snd : A*B -> B).
 Proof.
   intros p1 p2 Rp. destruct Rp.
   split; eapply Proper_snd; assumption.
@@ -223,29 +223,29 @@ Qed.
  ***)
 
 (* The type of continuous, i.e. Proper, functions between ordered types *)
-Record Pfun A B {RA:OType A} {RB:OType B} :=
+Record Ofun A B {RA:OType A} {RB:OType B} :=
   {
-    pfun_app : A -> B;
-    pfun_Proper : Proper (ot_R ==> ot_R) pfun_app
+    ofun_app : A -> B;
+    ofun_Proper : Proper (oleq ==> oleq) ofun_app
   }.
 
-Arguments pfun_app {_ _ _ _} _ _.
-Arguments pfun_Proper [_ _ _ _] _ _ _ _.
+Arguments ofun_app {_ _ _ _} _ _.
+Arguments ofun_Proper [_ _ _ _] _ _ _ _.
 
 Notation "A '-o>' B" :=
-  (Pfun A B) (right associativity, at level 99).
+  (Ofun A B) (right associativity, at level 99).
 Notation "x @o@ y" :=
-  (pfun_app x y) (left associativity, at level 20).
+  (ofun_app x y) (left associativity, at level 20).
 
 (* The non-dependent function ordered type *)
 Instance OTarrow A B `{OType A} `{OType B} : OType (A -o> B) :=
-  {| ot_R :=
+  {| oleq :=
        fun f g =>
-         forall a1 a2, ot_R a1 a2 -> ot_R (pfun_app f a1) (pfun_app g a2) |}.
+         forall a1 a2, oleq a1 a2 -> oleq (ofun_app f a1) (ofun_app g a2) |}.
 Proof.
   repeat constructor; intro; intros.
-  { apply pfun_Proper; assumption. }
-  { transitivity (pfun_app y a1).
+  { apply ofun_Proper; assumption. }
+  { transitivity (ofun_app y a1).
     - apply H1; reflexivity.
     - apply H2; assumption. }
 Defined.
@@ -255,136 +255,136 @@ Defined.
 itself be proper, i.e., to be an element of OTarrow A OType. *)
 
 
-(* pfun_app is always Proper *)
-Instance Proper_pfun_app A B `{OType A} `{OType B} :
-  Proper (ot_R ==> ot_R ==> ot_R) (@pfun_app A B _ _).
+(* ofun_app is always Proper *)
+Instance Proper_ofun_app A B `{OType A} `{OType B} :
+  Proper (oleq ==> oleq ==> oleq) (@ofun_app A B _ _).
 Proof.
   intros f1 f2 Rf a1 a2 Ra. apply Rf; assumption.
 Qed.
 
-(* pfun_app is always Proper w.r.t. ot_equiv *)
-Instance Proper_pfun_app_equiv A B `{OType A} `{OType B} :
-  Proper (ot_equiv ==> ot_equiv ==> ot_equiv) (@pfun_app A B _ _).
+(* ofun_app is always Proper w.r.t. oeq *)
+Instance Proper_ofun_app_equiv A B `{OType A} `{OType B} :
+  Proper (oeq ==> oeq ==> oeq) (@ofun_app A B _ _).
 Proof.
   intros f1 f2 Rf a1 a2 Ra; destruct Rf; destruct Ra.
-  split; apply Proper_pfun_app; assumption.
+  split; apply Proper_ofun_app; assumption.
 Qed.
 
-Instance Proper_pfun_app_partial A B `{OType A} `{OType B} f :
-  Proper (ot_R ==> ot_R) (pfun_app (A:=A) (B:=B) f).
+Instance Proper_ofun_app_partial A B `{OType A} `{OType B} f :
+  Proper (oleq ==> oleq) (ofun_app (A:=A) (B:=B) f).
 Proof.
-  apply pfun_Proper.
+  apply ofun_Proper.
 Qed.
 
-Instance Proper_pfun_app_partial_equiv A B `{OType A} `{OType B} f :
-  Proper (ot_equiv ==> ot_equiv) (@pfun_app A B _ _ f).
+Instance Proper_ofun_app_partial_equiv A B `{OType A} `{OType B} f :
+  Proper (oeq ==> oeq) (@ofun_app A B _ _ f).
 Proof.
-  intros a1 a2 Ra; destruct Ra; split; apply pfun_Proper; assumption.
+  intros a1 a2 Ra; destruct Ra; split; apply ofun_Proper; assumption.
 Qed.
 
 
 (***
- *** Some Useful Pfuns
+ *** Some Useful Ofuns
  ***)
 
-(* The identity pfun *)
-Definition id_pfun {A} `{OType A} : A -o> A :=
-  {| pfun_app := fun x => x; pfun_Proper := fun x1 x2 Rx => Rx |}.
+(* The identity ofun *)
+Definition id_ofun {A} `{OType A} : A -o> A :=
+  {| ofun_app := fun x => x; ofun_Proper := fun x1 x2 Rx => Rx |}.
 
-(* The identity pfun *)
-Program Definition compose_pfun {A B C}
+(* The identity ofun *)
+Program Definition compose_ofun {A B C}
         `{OType A} `{OType B} `{OType C}
         (f:A -o> B) (g:B -o> C) : A -o> C :=
-  {| pfun_app := fun x => pfun_app g (pfun_app f x);
-     pfun_Proper := _ |}.
+  {| ofun_app := fun x => ofun_app g (ofun_app f x);
+     ofun_Proper := _ |}.
 Next Obligation.
-  intros x1 x2 Rx. apply pfun_Proper. apply pfun_Proper. assumption.
+  intros x1 x2 Rx. apply ofun_Proper. apply ofun_Proper. assumption.
 Qed.
 
-Instance Proper_compose_pfun A B C
+Instance Proper_compose_ofun A B C
          `{OType A} `{OType B} `{OType C} :
-  Proper (ot_R ==> ot_R ==> ot_R) (@compose_pfun A B C _ _ _).
+  Proper (oleq ==> oleq ==> oleq) (@compose_ofun A B C _ _ _).
   intros f1 f2 Rf g1 g2 Rg a1 a2 Ra.
   apply Rg. apply Rf. assumption.
 Qed.
 
-Instance Proper_compose_pfun_equiv A B C
+Instance Proper_compose_ofun_equiv A B C
          `{OType A} `{OType B} `{OType C} :
-  Proper (ot_equiv ==> ot_equiv ==> ot_equiv) (@compose_pfun A B C _ _ _).
+  Proper (oeq ==> oeq ==> oeq) (@compose_ofun A B C _ _ _).
 Proof.
   intros f1 f2 Rf g1 g2 Rg.
   split; intros a1 a2 Ra; simpl; apply Rg; apply Rf; apply Ra.
 Qed.
 
-(* Category theory laws for Pfuns *)
-Lemma id_compose_pfun A B `{OType A} `{OType B} (f: A -o> B) :
-  ot_equiv (compose_pfun id_pfun f) f.
-  split; intros a1 a2 Ra; simpl; apply pfun_Proper; assumption.
+(* Category theory laws for Ofuns *)
+Lemma id_compose_ofun A B `{OType A} `{OType B} (f: A -o> B) :
+  oeq (compose_ofun id_ofun f) f.
+  split; intros a1 a2 Ra; simpl; apply ofun_Proper; assumption.
 Qed.
-Lemma compose_id_pfun A B `{OType A} `{OType B} (f: A -o> B) :
-  ot_equiv (compose_pfun f id_pfun) f.
-  split; intros a1 a2 Ra; simpl; apply pfun_Proper; assumption.
+Lemma compose_id_ofun A B `{OType A} `{OType B} (f: A -o> B) :
+  oeq (compose_ofun f id_ofun) f.
+  split; intros a1 a2 Ra; simpl; apply ofun_Proper; assumption.
 Qed.
-Lemma compose_compose_pfun A B C D
+Lemma compose_compose_ofun A B C D
       `{OType A} `{OType B} `{OType C} `{OType D}
       (f: A -o> B) (g: B -o> C) (h: C -o> D) :
-  ot_equiv (compose_pfun f (compose_pfun g h)) (compose_pfun (compose_pfun f g) h).
-  split; intros a1 a2 Ra; simpl; repeat apply pfun_Proper; assumption.
+  oeq (compose_ofun f (compose_ofun g h)) (compose_ofun (compose_ofun f g) h).
+  split; intros a1 a2 Ra; simpl; repeat apply ofun_Proper; assumption.
 Qed.
 
-(* The constant pfun *)
-Program Definition const_pfun {A B} `{OType A} `{OType B} b : A -o> B :=
-  {| pfun_app := fun _ => b; pfun_Proper := fun _ _ _ => ltac:(reflexivity) |}.
+(* The constant ofun *)
+Program Definition const_ofun {A B} `{OType A} `{OType B} b : A -o> B :=
+  {| ofun_app := fun _ => b; ofun_Proper := fun _ _ _ => ltac:(reflexivity) |}.
 
 (* FIXME: this proper-ness proof should include irrelevance of the OType arg *)
-Instance Proper_const_pfun {A B} `{OType A} `{OType B} :
-  Proper (ot_R ==> ot_R) (const_pfun (A:=A) (B:=B)).
+Instance Proper_const_ofun {A B} `{OType A} `{OType B} :
+  Proper (oleq ==> oleq) (const_ofun (A:=A) (B:=B)).
 Proof.
   intros b1 b2 Rb a1 a2 Ra. apply Rb.
 Qed.
 
-Instance Proper_const_pfun_equiv {A B} `{OType A} `{OType B} :
-  Proper (ot_equiv ==> ot_equiv) (const_pfun (A:=A) (B:=B)).
+Instance Proper_const_ofun_equiv {A B} `{OType A} `{OType B} :
+  Proper (oeq ==> oeq) (const_ofun (A:=A) (B:=B)).
 Proof.
   intros b1 b2 Rb; split; intros a1 a2 Ra; apply Rb.
 Qed.
 
-(* Composing with the constant pfun on the left *)
-Lemma compose_const_pfun_f A B C `{OType A} `{OType B} `{OType C}
+(* Composing with the constant ofun on the left *)
+Lemma compose_const_ofun_f A B C `{OType A} `{OType B} `{OType C}
       b (f : B -o> C) :
-  ot_equiv (compose_pfun (const_pfun (A:=A) b) f) (const_pfun (pfun_app f b)).
+  oeq (compose_ofun (const_ofun (A:=A) b) f) (const_ofun (ofun_app f b)).
   split; intros a1 a2 Ra; reflexivity.
 Qed.
 
-(* Composing with the constant pfun on the right *)
-Lemma compose_f_const_pfun A B C `{OType A} `{OType B} `{OType C}
+(* Composing with the constant ofun on the right *)
+Lemma compose_f_const_ofun A B C `{OType A} `{OType B} `{OType C}
       (f : A -o> B) c :
-  ot_equiv (compose_pfun f (const_pfun c)) (const_pfun c).
+  oeq (compose_ofun f (const_ofun c)) (const_ofun c).
   split; intros a1 a2 Ra; reflexivity.
 Qed.
 
 
-(* Take the pair of the outputs of two pfuns *)
-Program Definition pair_pfun {A B C}
+(* Take the pair of the outputs of two ofuns *)
+Program Definition pair_ofun {A B C}
         `{OType A} `{OType B} `{OType C}
         (f: A -o> B) (g: A -o> C) : A -o> (B * C) :=
-  {| pfun_app := fun a => (pfun_app f a, pfun_app g a) |}.
+  {| ofun_app := fun a => (ofun_app f a, ofun_app g a) |}.
 Next Obligation.
-  intros a1 a2 Ra; split; apply pfun_Proper; assumption.
+  intros a1 a2 Ra; split; apply ofun_Proper; assumption.
 Qed.
 
-Instance Proper_pair_pfun A B C `{OType A} `{OType B} `{OType C} :
-  Proper (ot_R ==> ot_R ==> ot_R) (pair_pfun (A:=A) (B:=B) (C:=C)).
+Instance Proper_pair_ofun A B C `{OType A} `{OType B} `{OType C} :
+  Proper (oleq ==> oleq ==> oleq) (pair_ofun (A:=A) (B:=B) (C:=C)).
 Proof.
   intros a1 a2 Ra b1 b2 Rb c1 c2 Rc; simpl; split.
   - apply Ra; assumption.
   - apply Rb; assumption.
 Qed.
 
-Instance Proper_pair_pfun_equiv A B C
+Instance Proper_pair_ofun_equiv A B C
          `{OType A} `{OType B} `{OType C} :
-  Proper (ot_equiv ==> ot_equiv ==> ot_equiv)
-         (pair_pfun (A:=A) (B:=B) (C:=C)).
+  Proper (oeq ==> oeq ==> oeq)
+         (pair_ofun (A:=A) (B:=B) (C:=C)).
 Proof.
   intros a1 a2 Ra b1 b2 Rb.
   destruct Ra as [ Ra1 Ra2 ]; destruct Rb as [ Rb1 Rb2 ].
@@ -393,197 +393,197 @@ Proof.
 Qed.
 
 (* compose commutes with pair *)
-Lemma compose_f_pair_pfun A B C D
+Lemma compose_f_pair_ofun A B C D
       `{OType A} `{OType B} `{OType C} `{OType D}
       (f: A -o> B) (g: B -o> C) (h: B -o> D) :
-  ot_equiv (compose_pfun f (pair_pfun g h))
-           (pair_pfun (compose_pfun f g) (compose_pfun f h)).
-  split; intros a1 a2 Ra; simpl; split; repeat apply pfun_Proper; assumption.
+  oeq (compose_ofun f (pair_ofun g h))
+           (pair_ofun (compose_ofun f g) (compose_ofun f h)).
+  split; intros a1 a2 Ra; simpl; split; repeat apply ofun_Proper; assumption.
 Qed.
 
-(* The first projection pfun *)
-Definition fst_pfun {A B} `{OType A} `{OType B} : A * B -o> A :=
-  {| pfun_app := fst; pfun_Proper := _ |}.
+(* The first projection ofun *)
+Definition fst_ofun {A B} `{OType A} `{OType B} : A * B -o> A :=
+  {| ofun_app := fst; ofun_Proper := _ |}.
 
-(* The second projection pfun *)
-Definition snd_pfun {A B} `{OType A} `{OType B} : A * B -o> B :=
-  {| pfun_app := snd; pfun_Proper := _ |}.
+(* The second projection ofun *)
+Definition snd_ofun {A B} `{OType A} `{OType B} : A * B -o> B :=
+  {| ofun_app := snd; ofun_Proper := _ |}.
 
 (* Composing pair with fst gives the first function in the pair *)
 Lemma compose_pair_fst A B C `{OType A} `{OType B} `{OType C}
       (f: A -o> B) (g: A -o> C) :
-  ot_equiv (compose_pfun (pair_pfun f g) fst_pfun) f.
-  split; intros a1 a2 Ra; simpl; apply pfun_Proper; assumption.
+  oeq (compose_ofun (pair_ofun f g) fst_ofun) f.
+  split; intros a1 a2 Ra; simpl; apply ofun_Proper; assumption.
 Qed.
 
 (* Composing pair with snd gives the second function in the pair *)
 Lemma compose_pair_snd A B C `{OType A} `{OType B} `{OType C}
       (f: A -o> B) (g: A -o> C) :
-  ot_equiv (compose_pfun (pair_pfun f g) snd_pfun) g.
-  split; intros a1 a2 Ra; simpl; apply pfun_Proper; assumption.
+  oeq (compose_ofun (pair_ofun f g) snd_ofun) g.
+  split; intros a1 a2 Ra; simpl; apply ofun_Proper; assumption.
 Qed.
 
 (* Taking the pair of fst and snd is the identity *)
 Lemma pair_fst_snd_eta A B `{OType A} `{OType B} :
-  ot_equiv (pair_pfun (fst_pfun (A:=A) (B:=B)) snd_pfun) id_pfun.
+  oeq (pair_ofun (fst_ofun (A:=A) (B:=B)) snd_ofun) id_ofun.
   split; intros p1 p2 Rp; destruct Rp; split; simpl; assumption.
 Qed.
 
 
-(* Curry a Pfun *)
-Program Definition pfun_curry {A B C} `{OType A} `{OType B} `{OType C}
-        (pfun : (A * B) -o> C)
+(* Curry a Ofun *)
+Program Definition ofun_curry {A B C} `{OType A} `{OType B} `{OType C}
+        (ofun : (A * B) -o> C)
   : A -o> (B -o> C) :=
-  {| pfun_app :=
+  {| ofun_app :=
        fun a =>
-         {| pfun_app := fun b => pfun_app pfun (a,b);
-            pfun_Proper := _ |};
-     pfun_Proper := _ |}.
+         {| ofun_app := fun b => ofun_app ofun (a,b);
+            ofun_Proper := _ |};
+     ofun_Proper := _ |}.
 Next Obligation.
 Proof.
-  intros b1 b2 Rb. apply pfun_Proper.
+  intros b1 b2 Rb. apply ofun_Proper.
   split; [ reflexivity | assumption ].
 Qed.
 Next Obligation.
 Proof.
   intros a1 a2 Ra b1 b2 Rb; simpl.
-  apply pfun_Proper; split; assumption.
+  apply ofun_Proper; split; assumption.
 Qed.
 
-(* Uncrry a Pfun *)
-Program Definition pfun_uncurry {A B C}
+(* Uncrry a Ofun *)
+Program Definition ofun_uncurry {A B C}
         `{OType A} `{OType B} `{OType C}
-        (pfun : A -o> (B -o> C))
+        (ofun : A -o> (B -o> C))
   : (A * B) -o> C :=
-  {| pfun_app :=
-       fun ab => pfun_app (pfun_app pfun (fst ab)) (snd ab);
-     pfun_Proper := _ |}.
+  {| ofun_app :=
+       fun ab => ofun_app (ofun_app ofun (fst ab)) (snd ab);
+     ofun_Proper := _ |}.
 Next Obligation.
 Proof.
   intros ab1 ab2 Rab. destruct Rab as [ Ra Rb ].
-  exact (pfun_Proper pfun (fst ab1) (fst ab2) Ra (snd ab1) (snd ab2) Rb).
+  exact (ofun_Proper ofun (fst ab1) (fst ab2) Ra (snd ab1) (snd ab2) Rb).
 Qed.
 
 
-(* pfun_curry is Proper *)
-Instance Proper_pfun_curry A B C `{OType A} `{OType B} `{OType C}
-  : Proper (ot_R ==> ot_R) (pfun_curry (A:=A) (B:=B) (C:=C)).
+(* ofun_curry is Proper *)
+Instance Proper_ofun_curry A B C `{OType A} `{OType B} `{OType C}
+  : Proper (oleq ==> oleq) (ofun_curry (A:=A) (B:=B) (C:=C)).
 Proof.
   intros f1 f2 Rf a1 a2 Ra b1 b2 Rb. apply Rf. split; assumption.
 Qed.
 
-(* pfun_curry is Proper w.r.t. equivalence *)
-Instance Proper_pfun_curry_equiv A B C `{OType A} `{OType B} `{OType C} :
-  Proper (ot_equiv ==> ot_equiv) (pfun_curry (A:=A) (B:=B) (C:=C)).
+(* ofun_curry is Proper w.r.t. equivalence *)
+Instance Proper_ofun_curry_equiv A B C `{OType A} `{OType B} `{OType C} :
+  Proper (oeq ==> oeq) (ofun_curry (A:=A) (B:=B) (C:=C)).
 Proof.
-  intros f1 f2 Rf; destruct Rf; split; apply Proper_pfun_curry; assumption.
+  intros f1 f2 Rf; destruct Rf; split; apply Proper_ofun_curry; assumption.
 Qed.
 
-(* FIXME: Proper instance for pfun_uncurry *)
+(* FIXME: Proper instance for ofun_uncurry *)
 
-(* Currying and uncurrying of pfuns form an isomorphism: part 1 *)
-Lemma pfun_curry_uncurry_eq A B C `{OType A} `{OType B} `{OType C}
+(* Currying and uncurrying of ofuns form an isomorphism: part 1 *)
+Lemma ofun_curry_uncurry_eq A B C `{OType A} `{OType B} `{OType C}
       (f: (A * B) -o> C) :
-  pfun_uncurry (pfun_curry f) =o= f.
-  split; intros ab1 ab2 Rab; simpl; apply pfun_Proper;
+  ofun_uncurry (ofun_curry f) =o= f.
+  split; intros ab1 ab2 Rab; simpl; apply ofun_Proper;
     destruct Rab; split; assumption.
 Qed.
 
-(* Currying and uncurrying of pfuns form an isomorphism: part 2 *)
-Lemma pfun_uncurry_curry_eq A B C `{OType A} `{OType B} `{OType C}
+(* Currying and uncurrying of ofuns form an isomorphism: part 2 *)
+Lemma ofun_uncurry_curry_eq A B C `{OType A} `{OType B} `{OType C}
       (f: A -o> B -o> C) :
-  pfun_curry (pfun_uncurry f) =o= f.
-  split; intros a1 a2 Ra b1 b2 Rb; simpl; apply Proper_pfun_app;
-    try apply pfun_Proper; assumption.
+  ofun_curry (ofun_uncurry f) =o= f.
+  split; intros a1 a2 Ra b1 b2 Rb; simpl; apply Proper_ofun_app;
+    try apply ofun_Proper; assumption.
 Qed.
 
 
-(* The S combinator for pfuns (FIXME: do we need this?) *)
-Program Definition pfun_S {A B C} `{OType A} `{OType B} `{OType C}
+(* The S combinator for ofuns (FIXME: do we need this?) *)
+Program Definition ofun_S {A B C} `{OType A} `{OType B} `{OType C}
   : (A -o> B -o> C) -o> (A -o> B) -o> A -o> C :=
-  {| pfun_app :=
+  {| ofun_app :=
        fun f =>
-         {| pfun_app :=
+         {| ofun_app :=
               fun g =>
-                {| pfun_app := fun a => pfun_app (pfun_app f a) (pfun_app g a) |}
+                {| ofun_app := fun a => ofun_app (ofun_app f a) (ofun_app g a) |}
          |}
   |}.
 Next Obligation.
-  intros a1 a2 Ra; apply Proper_pfun_app; try apply pfun_Proper; assumption.
+  intros a1 a2 Ra; apply Proper_ofun_app; try apply ofun_Proper; assumption.
 Qed.
 Next Obligation.
-  intros g1 g2 Rg a1 a2 Ra. simpl. apply Proper_pfun_app; try assumption.
-  - apply pfun_Proper; assumption.
+  intros g1 g2 Rg a1 a2 Ra. simpl. apply Proper_ofun_app; try assumption.
+  - apply ofun_Proper; assumption.
   - apply Rg; assumption.
 Qed.
 Next Obligation.
-  intros f1 f2 Rf g1 g2 Rg a1 a2 Ra. simpl. apply Proper_pfun_app; try assumption.
+  intros f1 f2 Rf g1 g2 Rg a1 a2 Ra. simpl. apply Proper_ofun_app; try assumption.
   - intros b1 b2 Rb. apply Rf; assumption.
   - apply Rg; assumption.
 Qed.
 
 (* This is the S combinator, but partially applied *)
-Program Definition pfun_apply {A B C}
+Program Definition ofun_apply {A B C}
         `{OType A} `{OType B} `{OType C}
         (f: A -o> B -o> C) (g: A -o> B) : A -o> C :=
-  {| pfun_app := fun a => pfun_app (pfun_app f a) (pfun_app g a) |}.
+  {| ofun_app := fun a => ofun_app (ofun_app f a) (ofun_app g a) |}.
 Next Obligation.
-  intros a1 a2 Ra; apply Proper_pfun_app; try apply pfun_Proper; assumption.
+  intros a1 a2 Ra; apply Proper_ofun_app; try apply ofun_Proper; assumption.
 Qed.
 
-Instance Proper_pfun_apply A B C `{OType A} `{OType B} `{OType C} :
-  Proper (ot_R ==> ot_R ==> ot_R) (pfun_apply (A:=A) (B:=B) (C:=C)).
+Instance Proper_ofun_apply A B C `{OType A} `{OType B} `{OType C} :
+  Proper (oleq ==> oleq ==> oleq) (ofun_apply (A:=A) (B:=B) (C:=C)).
 Proof.
   intros a1 a2 Ra b1 b2 Rb c1 c2 Rc. simpl.
   apply Ra; try assumption. apply Rb; try assumption.
 Qed.
 
-Instance Proper_pfun_apply_equiv A B C
+Instance Proper_ofun_apply_equiv A B C
          `{OType A} `{OType B} `{OType C} :
-  Proper (ot_equiv ==> ot_equiv ==> ot_equiv) (pfun_apply (A:=A) (B:=B) (C:=C)).
+  Proper (oeq ==> oeq ==> oeq) (ofun_apply (A:=A) (B:=B) (C:=C)).
 Proof.
   intros a1 a2 Ra b1 b2 Rb; split; intros c1 c2 Rc; simpl;
     apply Ra; try apply Rb; assumption.
 Qed.
 
 (* compose commutes with S *)
-Lemma compose_pfun_apply A B C D `{OType A} `{OType B} `{OType C} `{OType D}
+Lemma compose_ofun_apply A B C D `{OType A} `{OType B} `{OType C} `{OType D}
       (f : A -o> B) (g: B -o> C -o> D) h :
-  compose_pfun f (pfun_apply g h)
-  =o= pfun_apply (compose_pfun f g) (compose_pfun f h).
+  compose_ofun f (ofun_apply g h)
+  =o= ofun_apply (compose_ofun f g) (compose_ofun f h).
   split; intros a1 a2 Ra; simpl; rewrite Ra; reflexivity.
 Qed.
 
 (* compose commutes with currying *)
-Lemma compose_pfun_curry A B C D `{OType A} `{OType B} `{OType C} `{OType D}
+Lemma compose_ofun_curry A B C D `{OType A} `{OType B} `{OType C} `{OType D}
       (f: A -o> B) (g: B * C -o> D) :
-  ot_equiv (compose_pfun f (pfun_curry g))
-           (pfun_curry
-              (compose_pfun (pair_pfun (compose_pfun fst_pfun f) snd_pfun) g)).
+  oeq (compose_ofun f (ofun_curry g))
+           (ofun_curry
+              (compose_ofun (pair_ofun (compose_ofun fst_ofun f) snd_ofun) g)).
   split; intros a1 a2 Ra c1 c2 Rc; simpl; rewrite Ra; rewrite Rc; reflexivity.
 Qed.
 
 (* Applying a const is just composition. Note that we add the extra OType
 constraint to quantify over all possible proofs that B -o> C is an OType, so
 this rule applies independently of this aOType proof. *)
-Lemma pfun_apply_const A B C `{OType A} `{OType B} `{OType C}
+Lemma ofun_apply_const A B C `{OType A} `{OType B} `{OType C}
       {OBC: OType (B -o> C)} (f: B -o> C) (g: A -o> B) :
-  ot_equiv (pfun_apply (A:=A) (const_pfun f) g) (compose_pfun g f).
+  oeq (ofun_apply (A:=A) (const_ofun f) g) (compose_ofun g f).
   split; intros a1 a2 Ra; simpl; rewrite Ra; reflexivity.
 Qed.
 
-(* We can simplify pfun_S used with pfun_curry *)
-Lemma pfun_apply_pfun_curry A B C `{OType A} `{OType B} `{OType C} f g :
-  ot_equiv (pfun_apply (A:=A) (B:=B) (C:=C) (pfun_curry f) g)
-           (compose_pfun (pair_pfun id_pfun g) f).
-  split; intros a1 a2 Ra; simpl; apply pfun_Proper; split;
-    try apply pfun_Proper; assumption.
+(* We can simplify ofun_S used with ofun_curry *)
+Lemma ofun_apply_ofun_curry A B C `{OType A} `{OType B} `{OType C} f g :
+  oeq (ofun_apply (A:=A) (B:=B) (C:=C) (ofun_curry f) g)
+           (compose_ofun (pair_ofun id_ofun g) f).
+  split; intros a1 a2 Ra; simpl; apply ofun_Proper; split;
+    try apply ofun_Proper; assumption.
 Qed.
 
-(* The pair constructor as a pfun *)
-Program Definition pair_ctor_pfun {A B} `{OType A} `{OType B}
+(* The pair constructor as a ofun *)
+Program Definition pair_ctor_ofun {A B} `{OType A} `{OType B}
   : A -o> B -o> A * B :=
-  {| pfun_app := fun a => {| pfun_app := fun b => (a,b) |} |}.
+  {| ofun_app := fun a => {| ofun_app := fun b => (a,b) |} |}.
 Next Obligation.
   intros b1 b2 Rb; rewrite Rb; split; reflexivity.
 Qed.
@@ -591,11 +591,11 @@ Next Obligation.
   intros a1 a2 Ra b1 b2 Rb; simpl; rewrite Ra; rewrite Rb; split; reflexivity.
 Qed.
 
-(* Applying pair_ctor_pfun yields a pair_pfun *)
-Lemma apply_pair_ctor_pfun {A B C} `{OType A} `{OType B} `{OType C}
+(* Applying pair_ctor_ofun yields a pair_ofun *)
+Lemma apply_pair_ctor_ofun {A B C} `{OType A} `{OType B} `{OType C}
       (f: A -o> B) (g: A -o> C) :
-  ot_equiv (pfun_apply (pfun_apply (const_pfun pair_ctor_pfun) f) g)
-           (pair_pfun f g).
+  oeq (ofun_apply (ofun_apply (const_ofun pair_ctor_ofun) f) g)
+           (pair_ofun f g).
   split; intros a1 a2 Ra; simpl; rewrite Ra; split; reflexivity.
 Qed.
 
@@ -605,22 +605,22 @@ Qed.
  ***)
 
 Class ProperPair A `{OType A} (x y:A) : Prop :=
-  proper_pair_pf : ot_R x y.
+  proper_pair_pf : oleq x y.
 
-Class PFunProper {A B} `{OType A} `{OType B} (f: A -> B) : Prop :=
-  pfun_proper : forall x y, ProperPair A x y -> ProperPair B (f x) (f y).
+Class OFunProper {A B} `{OType A} `{OType B} (f: A -> B) : Prop :=
+  ofun_proper : forall x y, ProperPair A x y -> ProperPair B (f x) (f y).
 
-Hint Extern 1 (PFunProper _) => intro; intro; intro : typeclass_instances.
+Hint Extern 1 (OFunProper _) => intro; intro; intro : typeclass_instances.
 
-Definition mk_pfun {A B} `{OType A} `{OType B} (f: A -> B) {prp:PFunProper f}
+Definition mk_ofun {A B} `{OType A} `{OType B} (f: A -> B) {prp:OFunProper f}
   : A -o> B :=
-  {| pfun_app := f; pfun_Proper := prp |}.
+  {| ofun_app := f; ofun_Proper := prp |}.
 
-Notation "'pfun' x => e" := (mk_pfun (fun x => e))
+Notation "'ofun' x => e" := (mk_ofun (fun x => e))
                               (right associativity, at level 99).
 
-Notation "'pfun' ( x : A ) => e" :=
-  (mk_pfun (fun x:A => e))
+Notation "'ofun' ( x : A ) => e" :=
+  (mk_ofun (fun x:A => e))
     (right associativity, at level 99, x at level 0).
 
 Instance ProperPair_refl A `{OType A} (x:A) : ProperPair A x x.
@@ -628,40 +628,40 @@ Proof.
   unfold ProperPair. reflexivity.
 Qed.
 
-Lemma ProperPair_pfun_app A B `{OType A} `{OType B}
+Lemma ProperPair_ofun_app A B `{OType A} `{OType B}
       (fl fr:A -o> B) argl argr
       (prpf:ProperPair (A -o> B) fl fr)
       (prpa:ProperPair A argl argr)
- : ProperPair B (pfun_app fl argl) (pfun_app fr argr).
+ : ProperPair B (ofun_app fl argl) (ofun_app fr argr).
 Proof.
   apply prpf; assumption.
 Qed.
 
-Lemma ProperPair_pfun A B `{OType A} `{OType B} (f g:A -> B) prpl prpr
+Lemma ProperPair_ofun A B `{OType A} `{OType B} (f g:A -> B) prpl prpr
          (pf: forall x y, ProperPair A x y -> ProperPair B (f x) (g y)) :
-  ProperPair (A -o> B) (@mk_pfun A B _ _ f prpl) (@mk_pfun A B _ _ g prpr).
+  ProperPair (A -o> B) (@mk_ofun A B _ _ f prpl) (@mk_ofun A B _ _ g prpr).
 Proof.
   intros xl xr Rx; apply pf; assumption.
 Qed.
 
 Hint Extern 2 (ProperPair _ _ _) =>
-first [ apply ProperPair_pfun_app
-      | apply ProperPair_pfun; do 3 intro ] : typeclass_instances.
+first [ apply ProperPair_ofun_app
+      | apply ProperPair_ofun; do 3 intro ] : typeclass_instances.
 
 (*
 Hint Extern 3 (ProperPair _ _ _) =>
 lazymatch goal with
-| |- ProperPair _ (pfun_app _ _) (pfun_app _ _) =>
-  apply ProperPair_pfun_app
+| |- ProperPair _ (ofun_app _ _) (ofun_app _ _) =>
+  apply ProperPair_ofun_app
 | |- ProperPair ?A (?f ?x) (?g ?y) =>
   let fapp := (eval beta in (f x)) in
   let gapp := (eval beta in (g y)) in
   change (ProperPair A fapp gapp)
-| |- ProperPair (?A -o> ?B) (@pfun _ _ _ _ ?f ?prpf) (@pfun _ _ _ _ ?g ?prpg) =>
+| |- ProperPair (?A -o> ?B) (@ofun _ _ _ _ ?f ?prpf) (@ofun _ _ _ _ ?g ?prpg) =>
   let x := fresh "x" in
   let y := fresh "y" in
   let ppair := fresh "ppair" in
-  apply ProperPair_pfun; intros x y ppair;
+  apply ProperPair_ofun; intros x y ppair;
     let fapp := eval beta in (f x) in
     let gapp := eval beta in (g y) in
     change (ProperPair B fapp gapp)
@@ -674,18 +674,18 @@ end.
 
 (* Proper function for fst *)
 Definition ofst {A B} `{OType A} `{OType B} : A * B -o> A :=
-  {| pfun_app := fst; pfun_Proper := _ |}.
+  {| ofun_app := fst; ofun_Proper := _ |}.
 
 (* Proper function for snd *)
 Definition osnd {A B} `{OType A} `{OType B} : A * B -o> B :=
-  {| pfun_app := snd; pfun_Proper := _ |}.
+  {| ofun_app := snd; ofun_Proper := _ |}.
 
 (* Proper function for pair *)
 Program Definition opair {A B} `{OType A} `{OType B} : A -o> B -o> A * B :=
-  {| pfun_app :=
-       fun a => {| pfun_app := fun b => pair a b;
-                   pfun_Proper := _ |};
-     pfun_Proper := _ |}.
+  {| ofun_app :=
+       fun a => {| ofun_app := fun b => pair a b;
+                   ofun_Proper := _ |};
+     ofun_Proper := _ |}.
 Next Obligation.
   intros b1 b2 Rb. split; [ reflexivity | assumption ].
 Qed.
@@ -699,7 +699,7 @@ Notation "( x ,o, y )" := (opair @o@ x @o@ y) (at level 0).
 (* FIXME: get this notation to work *)
 (*
 Notation "( x ,o, y ,o, .. ,o, z )" :=
-  (pfun_app opair .. (pfun_app (pfun_app opair x) y) .. z)
+  (ofun_app opair .. (ofun_app (ofun_app opair x) y) .. z)
                                          (at level 0).
 *)
 
@@ -733,14 +733,14 @@ Qed.
 
 (* Proper function for inl *)
 Program Definition oinl {A B} `{OType A} `{OType B} : A -o> A + B :=
-  {| pfun_app := inl; pfun_Proper := _ |}.
+  {| ofun_app := inl; ofun_Proper := _ |}.
 Next Obligation.
   intros x y Rxy. left. assumption.
 Defined.
 
 (* Proper function for inr *)
 Program Definition oinr {A B} `{OType A} `{OType B} : B -o> A + B :=
-  {| pfun_app := inr; pfun_Proper := _ |}.
+  {| ofun_app := inr; ofun_Proper := _ |}.
 Next Obligation.
   intros x y Rxy. right. assumption.
 Defined.
@@ -748,21 +748,21 @@ Defined.
 (* Proper function for eliminating sums *)
 Program Definition osum_elim {A B C} `{OType A} `{OType B} `{OType C} :
   (A -o> C) -o> (B -o> C) -o> A + B -o> C :=
-  {| pfun_app :=
+  {| ofun_app :=
        fun f1 =>
-         {| pfun_app :=
+         {| ofun_app :=
               fun f2 =>
-                {| pfun_app := fun (s : A+B) =>
+                {| ofun_app := fun (s : A+B) =>
                                  match s return C with
                                  | inl a => f1 @o@ a
                                  | inr b => f2 @o@ b
                                  end |} |} |}.
 Next Obligation.
-  intros s1 s2 Rs. destruct Rs; apply pfun_Proper; assumption.
+  intros s1 s2 Rs. destruct Rs; apply ofun_Proper; assumption.
 Defined.
 Next Obligation.
   intros f2 f2' Rf2 a1 a2 Ra. destruct Ra; simpl.
-  - apply pfun_Proper; assumption.
+  - apply ofun_Proper; assumption.
   - apply Rf2; assumption.
 Defined.
 Next Obligation.
@@ -772,7 +772,7 @@ Next Obligation.
 Defined.
 
 Lemma osum_elim_eta  {A B} `{OType A} `{OType B} :
-  osum_elim (A:=A) (B:=B) @o@ oinl @o@ oinr =o= id_pfun.
+  osum_elim (A:=A) (B:=B) @o@ oinl @o@ oinr =o= id_ofun.
 Proof.
   split; intros s1 s2 Rs; destruct Rs; simpl; constructor; assumption.
 Qed.
@@ -783,22 +783,22 @@ Qed.
  ***)
 
 Program Definition oif {A} `{OType A} : bool -o> A -o> A -o> A :=
-  mk_pfun
+  mk_ofun
     (fun (b:bool) =>
-       mk_pfun
+       mk_ofun
          (fun x =>
-            mk_pfun
+            mk_ofun
               (fun y => if b then x else y) (prp:=_)) (prp:=_)) (prp:=_).
 Next Obligation.
-  unfold PFunProper, ProperPair; intros a1 a2 Ra.
+  unfold OFunProper, ProperPair; intros a1 a2 Ra.
   destruct b; [ reflexivity | apply Ra ].
 Defined.
 Next Obligation.
-  unfold PFunProper, ProperPair; intros a1 a2 R12 a3 a4 R34.
+  unfold OFunProper, ProperPair; intros a1 a2 R12 a3 a4 R34.
   destruct b; [ apply R12 | assumption ].
 Defined.
 Next Obligation.
-  unfold PFunProper, ProperPair; simpl; intros.
+  unfold OFunProper, ProperPair; simpl; intros.
   destruct x; destruct y; try discriminate; assumption.
 Defined.
 
@@ -809,14 +809,14 @@ Defined.
 
 (* The universal combinator as an ordered function *)
 Program Definition oforall `{OType} : (A -o> Prop) -o> Prop :=
-  mk_pfun (fun (P:A -o> Prop) => forall x, P @o@ x) (prp:=_).
+  mk_ofun (fun (P:A -o> Prop) => forall x, P @o@ x) (prp:=_).
 Next Obligation.
   intros P1 P2 R12 pf z. apply (R12 _ _ (reflexivity _) (pf z)).
 Defined.
 
 (* The existential combinator as an ordered function *)
 Program Definition oexists `{OType} : (A -o> Prop) -o> Prop :=
-  mk_pfun (fun P => exists x, P @o@ x) (prp:=_).
+  mk_ofun (fun P => exists x, P @o@ x) (prp:=_).
 Next Obligation.
   intros P1 P2 R12 pf. destruct pf as [z pf].
   exists z. apply (R12 _ _ (reflexivity _) pf).
@@ -824,9 +824,9 @@ Defined.
 
 (* The double existential combinator as an ordered function *)
 Program Definition oexists2 `{OType} : (A -o> Prop) -o> (A -o> Prop) -o> Prop :=
-  mk_pfun
+  mk_ofun
     (fun P =>
-       mk_pfun
+       mk_ofun
          (fun Q => exists2 x, P @o@ x & Q @o@ x) (prp:=_)) (prp:=_).
 Next Obligation.
   intros P1 P2 R12 pf. destruct pf as [z pf1 pf2].
@@ -840,7 +840,7 @@ Defined.
 
 (* Conjunction as an ordered function *)
 Program Definition oand : Prop -o> Prop -o> Prop :=
-  mk_pfun (fun P1 => mk_pfun (fun P2 => P1 /\ P2) (prp:=_)) (prp:=_).
+  mk_ofun (fun P1 => mk_ofun (fun P2 => P1 /\ P2) (prp:=_)) (prp:=_).
 Next Obligation.
   intros P2' P2'' R2 H0. destruct H0; split; try assumption.
   apply R2; assumption.
@@ -852,7 +852,7 @@ Defined.
 
 (* Disjunction as an ordered function *)
 Program Definition oor : Prop -o> Prop -o> Prop :=
-  mk_pfun (fun P1 => mk_pfun (fun P2 => P1 \/ P2) (prp:=_)) (prp:=_).
+  mk_ofun (fun P1 => mk_ofun (fun P2 => P1 \/ P2) (prp:=_)) (prp:=_).
 Next Obligation.
   intros P2' P2'' R2 H0.
   destruct H0; [ left | right; apply R2 ]; assumption.
@@ -864,8 +864,8 @@ Defined.
 
 (* Implication as an ordered function *)
 Program Definition oimpl : Flip Prop -o> Prop -o> Prop :=
-  mk_pfun (fun (P1:Flip Prop) =>
-             mk_pfun (fun (P2:Prop) =>
+  mk_ofun (fun (P1:Flip Prop) =>
+             mk_ofun (fun (P2:Prop) =>
                         unflip P1 -> P2) (prp:=_)) (prp:=_).
 Next Obligation.
   intros P2 P2' R2 pf12 pf1.
@@ -878,8 +878,8 @@ Defined.
 
 (* Ordered type relations are themselves ordered propositional functions *)
 Program Definition oR `{OType} : Flip A -o> A -o> Prop :=
-  mk_pfun (fun (x:Flip A) =>
-             mk_pfun (fun y => ot_R (unflip x) y) (prp:=_)) (prp:=_).
+  mk_ofun (fun (x:Flip A) =>
+             mk_ofun (fun y => oleq (unflip x) y) (prp:=_)) (prp:=_).
 Next Obligation.
   intros a1 a2 Ra pf. etransitivity; eassumption.
 Defined.
@@ -896,11 +896,11 @@ Defined.
  ***)
 
 (* FIXME: why don't these work?
-Notation "'pfun' ( x : A ) =o> t" :=
+Notation "'ofun' ( x : A ) =o> t" :=
   (@ot_Lambda A _ (fun x => t))
     (at level 100, right associativity, x at level 99) : pterm_scope.
 
-Notation "'pfun' x =o> t" :=
+Notation "'ofun' x =o> t" :=
   (ot_Lambda (fun x => t))
     (at level 100, right associativity, x at level 99) : pterm_scope.
  *)
@@ -942,32 +942,32 @@ Ltac findOTypeF1 :=
 
 Module OTExamples.
 
-Definition ex1 : Prop -o> Prop := pfun p => p.
-(* Eval compute in (pfun_app ex1 : Prop -> Prop). *)
+Definition ex1 : Prop -o> Prop := ofun p => p.
+(* Eval compute in (ofun_app ex1 : Prop -> Prop). *)
 
-Definition ex2 {A} `{OType A} : A -o> A := pfun p => p.
-(* Eval simpl in (fun A `{OType A} => pfun_app (@ex2 A _ _) : A -> A). *)
+Definition ex2 {A} `{OType A} : A -o> A := ofun p => p.
+(* Eval simpl in (fun A `{OType A} => ofun_app (@ex2 A _ _) : A -> A). *)
 
 Definition ex3 {A} `{OType A} : A -o> A -o> A :=
-  pfun p1 => pfun p2 => p1.
-(* Eval simpl in (fun (A:OType) x => pfun_app (pfun_app (@ex3 A) x)). *)
+  ofun p1 => ofun p2 => p1.
+(* Eval simpl in (fun (A:OType) x => ofun_app (ofun_app (@ex3 A) x)). *)
 
 Definition ex4 {A B} `{OType A} `{OType B} : (A * B -o> A) :=
-  pfun p => ofst @o@ p.
+  ofun p => ofst @o@ p.
 (* Eval simpl in (fun {A B} `{OType A} `{OType B} =>
-                 pfun_app ex4 : A * B -> A). *)
+                 ofun_app ex4 : A * B -> A). *)
 
 Definition ex5 {A B} `{OType A} `{OType B} : A * B -o> B * A :=
-  pfun p => (osnd @o@ p ,o, ofst @o@ p).
+  ofun p => (osnd @o@ p ,o, ofst @o@ p).
 (* Eval simpl in (fun {A B} `{OType A} `{OType B} =>
-                 pfun_app ex5 : A * B -> B * A). *)
+                 ofun_app ex5 : A * B -> B * A). *)
 
 Definition ex6 {A B C} `{OType A} `{OType B} `{OType C} : A * B * C -o> C * A :=
-  pfun triple => (osnd @o@ triple ,o, ofst @o@ (ofst @o@ triple)).
+  ofun triple => (osnd @o@ triple ,o, ofst @o@ (ofst @o@ triple)).
 
 Definition ex7 {A B C} `{OType A} `{OType B} `{OType C}
   : (A * B -o> C) -o> C -o> A -o> B -o> C :=
-  pfun f => pfun c =>
-  pfun a => pfun b => f @o@ (a ,o, b).
+  ofun f => ofun c =>
+  ofun a => ofun b => f @o@ (a ,o, b).
 
 End OTExamples.
