theories/Reflection2/PredMonad.v
@@ -46,7 +46,7 @@ Class PredMonad M PM {FOM: OTypeF1 M} {FOPM: OTypeF1 PM}
       forall {A B} `{OType A} `{OType B} m f prp,
         liftP @o@ (bindM @o@ m @o@ f)
         =o= bindM @o@ (liftP @o@ m) @o@
-                  (mk_pfun (fun x => liftP @o@ (f @o@ x)) (prp:=prp));
+                  (mk_ofun (fun x => liftP @o@ (f @o@ x)) (prp:=prp));
 
     (* FIXME: need laws about how the combinators interact *)
   }.
@@ -65,18 +65,18 @@ Infix "|=" := satisfiesP (at level 80).
 
 (* Disjunction is definable in terms of the existential *)
 Definition orP `{PredMonadOps} `{OType} : PM A _ -o> PM A _ -o> PM A _ :=
-  pfun P1 => pfun P2 =>
-  existsP @o@ (pfun (b:bool) => oif @o@ b @o@ P1 @o@ P2).
+  ofun P1 => ofun P2 =>
+  existsP @o@ (ofun (b:bool) => oif @o@ b @o@ P1 @o@ P2).
 
 (* True and false, which correspond to top and bottom, respectively *)
 Definition trueP `{PredMonadOps} `{OType} : PM A _ :=
-  existsP @o@ (pfun pm => pm).
+  existsP @o@ (ofun pm => pm).
 Definition falseP `{PredMonadOps} `{OType} : PM A _ :=
-  forallP @o@ (pfun pm => pm).
+  forallP @o@ (ofun pm => pm).
 
 (* An assertion inside a predicate monad *)
 Program Definition assertP `{PredMonad} : Prop -o> PM unit _ :=
-  mk_pfun (fun (P:Prop) => existsP @o@ (pfun (pf:P) => trueP)) (prp:=_).
+  mk_ofun (fun (P:Prop) => existsP @o@ (ofun (pf:P) => trueP)) (prp:=_).
 Next Obligation.
   intros P1 P2 RP. apply predmonad_existsP_elim; intro pf1.
   assert P2 as pf2; [ apply RP; assumption | ].
@@ -87,10 +87,10 @@ Defined.
 (* An assumption made for the duration of a predicate monad *)
 Program Definition assumingP `{PredMonad} `{OType} :
   Flip Prop -o> PM A _ -o> PM A _ :=
-  mk_pfun
+  mk_ofun
     (fun (P:Flip Prop) =>
-       mk_pfun (fun (Q:PM A _) =>
-                  forallP @o@ (pfun (pf:unflip P) => Q)) (prp:=_))
+       mk_ofun (fun (Q:PM A _) =>
+                  forallP @o@ (ofun (pf:unflip P) => Q)) (prp:=_))
        (prp:=_).
 Next Obligation.
   intros Q1 Q2 RQ.
@@ -121,18 +121,18 @@ Instance FindOTypeF1_DownSetM : FindOTypeF1 DownSetM (fun _ _ => _) := I.
 (* An existential with both a positive and a negative component *)
 Program Definition oexists2' `{OType} : (A -o> Prop) -o>
                                         (Flip A -o> Prop) -o> Prop :=
-  mk_pfun
+  mk_ofun
     (fun P1 =>
-       mk_pfun
+       mk_ofun
          (fun P2 =>
             exists2 x, P1 @o@ x & P2 @o@ flip x) (prp:=_)) (prp:=_).
 Next Obligation.
-  unfold PFunProper, ProperPair; simpl; intros. intro pf.
+  unfold OFunProper, ProperPair; simpl; intros. intro pf.
   destruct pf as [z pf1 pf2].
   exists z; try assumption. apply (H0 _ _ (reflexivity _)). assumption.
 Defined.
 Next Obligation.
-  unfold PFunProper, ProperPair; simpl; intros. intro pf.
+  unfold OFunProper, ProperPair; simpl; intros. intro pf.
   destruct pf as [z pf1 pf2].
   exists z; [ apply (H0 _ _ (reflexivity _)) |
               apply (H1 _ _ (reflexivity _)) ]; assumption.
@@ -142,11 +142,11 @@ Defined.
 Instance MonadOps_DownSetM : MonadOps DownSetM :=
   {| returnM :=
        fun A _ =>
-         pfun (x:A) => pfun (y:Flip A) => oR @o@ y @o@ x;
+         ofun (x:A) => ofun (y:Flip A) => oR @o@ y @o@ x;
      bindM :=
        fun A B _ _ =>
-         (pfun m => pfun f => pfun (y:Flip B) =>
-          oexists2' @o@ (pfun x => f @o@ x @o@ y) @o@ m)
+         (ofun m => ofun f => ofun (y:Flip B) =>
+          oexists2' @o@ (ofun x => f @o@ x @o@ y) @o@ m)
   |}.
 
 Instance Monad_DownSetM : Monad DownSetM.
@@ -158,7 +158,7 @@ Proof.
     + simpl. exists x; try reflexivity. rewrite <- Ra. assumption.
   - simpl; split; intros a1 a2 Ra pf.
     + destruct pf as [ z pf1 pf2].
-      refine (pfun_Proper m _ _ _ _); [ | eassumption ].
+      refine (ofun_Proper m _ _ _ _); [ | eassumption ].
       etransitivity; try eassumption. apply pf1.
     + exists (unflip a1); try assumption.
       destruct a1. simpl. assumption.
@@ -177,10 +177,10 @@ Instance PredMonadOps_DownSetM : PredMonadOps Identity DownSetM :=
   {|
     forallP :=
       fun A B _ _ =>
-        pfun P => pfun b => oforall @o@ (pfun a => P @o@ a @o@ b);
+        ofun P => ofun b => oforall @o@ (ofun a => P @o@ a @o@ b);
     existsP :=
       fun A B _ _ =>
-        pfun P => pfun b => oexists @o@ (pfun a => P @o@ a @o@ b);
+        ofun P => ofun b => oexists @o@ (ofun a => P @o@ a @o@ b);
     liftP :=
       fun A _ => returnM
   |}.
@@ -198,5 +198,5 @@ Proof.
       etransitivity; [ apply Rb | apply pf ].
     + destruct pf. simpl in * |- *. etransitivity; try eassumption.
       etransitivity; try eassumption.
-      apply pfun_Proper; assumption.
+      apply ofun_Proper; assumption.
 Qed.
